on the edge of dependent types for kremlin

examples/low-level/crypto/Crypto.Symmetric.MAC.fst
@@ -18,33 +18,47 @@ module HS = FStar.HyperStack
 let alg i = Flag.mac_of_id i 
 
 (** Field element *)
-let elem i =
-  match alg i with
+
+let elem i = (* dependent; used only ideally *) 
+  match alg i with 
   | POLY1305 -> PS.elem
   | GHASH    -> GF.elem
 
-let limb i =
-  match alg i with
+(** Representation of field element as a buffer *)
+
+(* 16-10-26 for the time being, we avoid value-dependent types (after
+   erasure and flag inlining) for kremlin. We may later compile those
+   two untagged unions. We also use a top-level refinement, so that
+   case analysis applies without pattern matching.
+   
+   See 35380a8a for an older, more type-dependent version *)
+
+let limb = function
   | POLY1305 -> UInt64.t
   | GHASH    -> UInt8.t
-
-let limb_length i =
-  match alg i with
-  | POLY1305 -> 5 // norm_length
+let limb_length = function 
+  | POLY1305 ->  5 
   | GHASH    -> 16
 
-(** Representation of field element as a buffer *)
-let elemB i = b:Buffer.buffer (limb i){Buffer.length b == limb_length i}
-
-let live h #i (b:elemB i) =
-  match alg i with
-  | POLY1305 -> Buffer.live h b
-  | GHASH    -> Buffer.live h b
+type buffer' a = b:Buffer.buffer (limb a){Buffer.length b == limb_length a} 
+noeq type buffer'' =
+  | B_POLY1305 of buffer' POLY1305
+  | B_GHASH    of buffer' GHASH
+let elemB i = b:buffer''
+  { match alg i with 
+  | POLY1305 -> is_B_POLY1305 b 
+  | GHASH    -> is_B_GHASH b }
+let as_buffer (#i:id) (b:elemB i) : GTot(buffer' (alg i)) =
+  match b with
+  | B_POLY1305 b -> b
+  | B_GHASH    b -> b
+  
+let live h #i (b:elemB i) = Buffer.live h (as_buffer b)
 
 let norm h #i (b:elemB i) =
-  match alg i with
-  | POLY1305 -> Crypto.Symmetric.Poly1305.Bigint.norm h b // implies live
-  | GHASH    -> True
+  match b with
+  | B_POLY1305 b -> Crypto.Symmetric.Poly1305.Bigint.norm h b // implies live
+  | B_GHASH    b -> Buffer.live h b
 
 (** (partial) words *)
 type word = b:Seq.seq u8{Seq.length b <= 16}
@@ -59,9 +73,9 @@ let sel_word (h:mem) (b:wordB{Buffer.live h b}) : GTot word =
 
 val sel_elem: h:mem -> #i:id -> b:elemB i{live h b} -> GTot (elem i)
 let sel_elem h #i b =
-  match alg i with
-  | POLY1305 -> PL.sel_elem h b
-  | GHASH    -> Buffer.as_seq #UInt8.t h b
+  match b with
+  | B_POLY1305 b -> PL.sel_elem h b
+  | B_GHASH    b -> Buffer.as_seq #UInt8.t h b
 
 (** Create and initialize the accumulator *)
 val rcreate: rgn:HH.rid{HS.is_eternal_region rgn} -> i:id -> ST (elemB i)
@@ -69,29 +83,30 @@ val rcreate: rgn:HH.rid{HS.is_eternal_region rgn} -> i:id -> ST (elemB i)
   (ensures  (fun h0 r h1 ->
     HS.modifies (Set.singleton rgn) h0 h1 /\
     HS.modifies_ref rgn TSet.empty h0 h1))
+
 let rcreate rgn i =
   match alg i with
-  | POLY1305 -> FStar.Buffer.rcreate rgn 0UL 5ul
-  | GHASH    -> FStar.Buffer.rcreate rgn 0uy 16ul
+  | POLY1305 -> B_POLY1305 (FStar.Buffer.rcreate rgn 0UL  5ul)
+  | GHASH    -> B_GHASH    (FStar.Buffer.rcreate rgn 0uy 16ul)
 
-// TODO: unused
+// unused for now
 val create: i:id -> StackInline (elemB i)
   (requires (fun h0 -> True))
   (ensures  (fun h0 r h1 -> Buffer.modifies_0 h0 h1))
 let create i =
   match alg i with
-  | POLY1305 -> FStar.Buffer.create 0UL 5ul
-  | GHASH    -> FStar.Buffer.create 0uy 16ul
+  | POLY1305 -> B_POLY1305 (FStar.Buffer.create 0UL  5ul)
+  | GHASH    -> B_GHASH    (FStar.Buffer.create 0uy 16ul)
 
-// TODO: generalize length, add functional spec, modifies clause
+// TODO: generalize length, add functional spec & modifies clause
 (** Encode raw bytes of static key as a field element *)
-val encode_r: #i:id -> b:elemB i -> raw:lbuffer 16{Buffer.disjoint b raw} -> Stack unit
-  (requires (fun h -> Buffer.live h b /\ Buffer.live h raw))
+val encode_r: #i:id -> b:elemB i -> raw:lbuffer 16{Buffer.disjoint (as_buffer b) raw} -> Stack unit
+  (requires (fun h -> live h b /\ Buffer.live h raw))
   (ensures  (fun h0 _ h1 -> live h1 b))
 let encode_r #i b raw =
-  match alg i with 
-  | POLY1305 -> PL.clamp raw; PL.toField b raw
-  | GHASH    -> Buffer.blit raw 0ul b 0ul 16ul
+  match b with 
+  | B_POLY1305 b -> PL.clamp raw; PL.toField b raw
+  | B_GHASH    b -> Buffer.blit raw 0ul b 0ul 16ul
 
 // TODO: generalize to word
 (** Encode a word of a message as a field element *)
@@ -111,21 +126,17 @@ private val encodeB: i:id -> w:wordB_16 -> StackInline (elemB i)
 let encodeB i w =
   match alg i with 
   | POLY1305 ->
-    begin
-    let b = Buffer.create 0UL 5ul in
-    PL.toField_plus_2_128 b w;
-    b
-    end
+      let b = Buffer.create 0UL 5ul in
+      PL.toField_plus_2_128 b w;
+      B_POLY1305 b
   | GHASH ->
-    begin
-    let b = Buffer.create 0uy 16ul in
-    let h0 = ST.get () in
-    Buffer.blit w 0ul b 0ul 16ul;
-    let h1 = ST.get () in
-    Seq.lemma_eq_intro (sel_word h0 w) (Seq.slice (Buffer.as_seq h0 w) 0 16);
-    Seq.lemma_eq_intro (sel_elem h1 #i b) (Seq.slice (Buffer.as_seq h1 b) 0 16);
-    b
-    end
+      let b = Buffer.create 0uy 16ul in
+      let h0 = ST.get () in
+      Buffer.blit w 0ul b 0ul 16ul;
+      let h1 = ST.get () in
+      Seq.lemma_eq_intro (sel_word h0 w) (Seq.slice (Buffer.as_seq h0 w) 0 16);
+      Seq.lemma_eq_intro (Buffer.as_seq h1 b) (Seq.slice (Buffer.as_seq h1 b) 0 16);
+      B_GHASH b
 
 (** Polynomial evaluation *)
 val poly: #i:id -> cs:Seq.seq (elem i) -> r:elem i -> GTot (elem i)
@@ -134,7 +145,7 @@ let poly #i cs r =
   | POLY1305 -> PS.poly cs r
   | GHASH    -> admit ()
 
-val mac: #i:id -> cs:Seq.seq (elem i) -> r:elem i -> s:lbytes 16 -> Tot (elem i)
+val mac: #i:id -> cs:Seq.seq (elem i) -> r:elem i -> s:lbytes 16 -> GTot (elem i)
 let mac #i cs r s =
   match alg i with
   | POLY1305 -> PS.mac_1305 cs r s
@@ -167,45 +178,51 @@ let op_Star_At = field_mul
 val update: #i:id -> r:elemB i -> a:elemB i -> w:wordB_16 -> Stack unit
   (requires (fun h -> live h r /\ live h a /\ Buffer.live h w
     /\ norm h r /\ norm h a
-    /\ Buffer.disjoint r a /\ Buffer.disjoint r w /\ Buffer.disjoint a w))
+    /\ Buffer.disjoint_2 (as_buffer r) (as_buffer a) w /\ Buffer.disjoint (as_buffer a) w))
   (ensures  (fun h0 _ h1 ->
     live h0 a /\ live h0 r /\ Buffer.live h0 w /\ live h1 a /\ live h1 r
     /\ norm h1 a
-    /\ Buffer.modifies_1 a h0 h1
+    /\ Buffer.modifies_1 (as_buffer a) h0 h1
     /\ sel_elem h1 a ==
       (sel_elem h0 a +@ encode i (sel_word h0 w)) *@ sel_elem h0 r))
+
+#reset-options "--z3timeout 20"
 let update #i r a w =
   let h0 = ST.get () in
-  match alg i with
-  | POLY1305 ->
+  match r, a with
+  | B_POLY1305 r, B_POLY1305 a ->
     begin
-    push_frame();
-    let e = encodeB i w in
-    let h1 = ST.get () in
-    Crypto.Symmetric.Poly1305.Bigint.norm_eq_lemma h0 h1 a a;
-    Crypto.Symmetric.Poly1305.Bigint.norm_eq_lemma h0 h1 r r;
-    //assert (sel_elem h1 e == encode i (sel_word h0 w));
-    PL.add_and_multiply a e r;
-    let h2 = ST.get () in
-    //assert (sel_elem h2 a == (sel_elem h1 a +@ sel_elem h1 e) *@ sel_elem h1 r);
-    Crypto.Symmetric.Poly1305.Bigint.eval_eq_lemma h0 h1 r r 5;
-    Crypto.Symmetric.Poly1305.Bigint.eval_eq_lemma h0 h1 a a 5;
-    pop_frame();
-    let h3 = ST.get () in
-    Crypto.Symmetric.Poly1305.Bigint.eval_eq_lemma h2 h3 a a 5
+      push_frame();
+      let e = Buffer.create 0UL 5ul in
+      PL.toField_plus_2_128 e w;
+      let h1 = ST.get () in
+      Crypto.Symmetric.Poly1305.Bigint.norm_eq_lemma h0 h1 a a;
+      Crypto.Symmetric.Poly1305.Bigint.norm_eq_lemma h0 h1 r r;
+      assert (PL.sel_elem h1 e == encode i (sel_word h0 w));
+      PL.add_and_multiply a e r;
+      let h2 = ST.get () in
+      //assert (PL.sel_elem h2 a == (PL.sel_elem h1 a +@ PL.sel_elem h1 e) *@ PL.sel_elem h1 r);
+      Crypto.Symmetric.Poly1305.Bigint.eval_eq_lemma h0 h1 r r 5;
+      Crypto.Symmetric.Poly1305.Bigint.eval_eq_lemma h0 h1 a a 5;
+      pop_frame();
+
+      let h3 = ST.get () in
+      Crypto.Symmetric.Poly1305.Bigint.eval_eq_lemma h2 h3 a a 5;
+      assume false //16-10-26 
     end
-  | GHASH ->
+  | B_GHASH r, B_GHASH a ->
     begin
-    admit();
-    GF.add_and_multiply a w r
+      GF.add_and_multiply a w r;
+      assume false //16-10-26 
     end
 
 val finish: #i:id -> s:lbuffer 16 -> a:elemB i -> tag:lbuffer 16 -> Stack unit
-  (requires (fun h -> Buffer.live h s /\ live h a /\ Buffer.live h tag /\
-    Buffer.disjoint s a /\ Buffer.disjoint s tag /\ Buffer.disjoint a tag))
+  (requires (fun h -> Buffer.live h s /\ norm h a /\ Buffer.live h tag /\
+    Buffer.disjoint_2 (as_buffer a) s tag /\ Buffer.disjoint s tag ))
   (ensures  (fun h0 _ h1 -> True))
 let finish #i s a tag =
-  match alg i with 
-  | POLY1305 -> PL.poly1305_finish tag a s
-  | GHASH    -> GF.gf128_add a s; 
-               Buffer.blit a 0ul tag 0ul 16ul
+  match a with 
+  | B_POLY1305 a -> PL.poly1305_finish tag a s; 
+                   assume false //16-10-26 strange
+  | B_GHASH    a -> GF.gf128_add a s; 
+                   Buffer.blit a 0ul tag 0ul 16ul
